feat: try to use Axiom to unify Z with Prop

qcp/ast/annotated_C/alpha_equiv.c
@@ -5,7 +5,7 @@ bool alpha_equiv(term *t1, term *t2)
 /*@ With term1 term2
       Require store_term(t1, term1) *
               store_term(t2, term2)
-      Ensure __return == term_eqn(term1, term2) && t1 == t1@pre && t2 == t2@pre
+      Ensure __return == term_alpha_eqn(term1, term2) && t1 == t1@pre && t2 == t2@pre
    && store_term(t1, term1) * store_term(t2, term2)
 */
 {
